Adjust maker tactics to not need arguments
The arguments to the various package making tactics are now carried in
the goal type.  This will make it easier to call the tactics from OCaml.

src/Language/IdentifiersGENERATEDProofs.v
@@ -32,8 +32,8 @@ Module Compilers.
 
       Import ProofTactic.Settings.
 
-      Definition package_proofs : @ProofGoalType.package_proofs _ _ package.
-      Proof. ProofTactic.prove_package_proofs IdentifiersBasicGENERATED.Compilers.package. Qed.
+      Definition package_proofs : @ProofGoalType.package_proofs_with_args Compilers.base Compilers.ident package IdentifiersBasicGENERATED.Compilers.package.
+      Proof. ProofTactic.prove_package_proofs. Qed.
     End ident.
   End pattern.
 End Compilers.
