src/Rewriter/Passes/ToFancyWithCasts.v
@@ -12,8 +12,8 @@ Module Compilers.
   Import Language.API.Compilers.
   Import Language.Wf.Compilers.
   Import Language.WfExtra.Compilers.
-  Import Rewriter.AllTactics.Compilers.RewriteRules.GoalType.
-  Import Rewriter.AllTacticsExtra.Compilers.RewriteRules.Tactic.
+  Import Rewriter.AllTacticsExtra.Compilers.RewriteRules.GoalType.
+  Import Rewriter.AllTactics.Compilers.RewriteRules.Tactic.
   Import Compilers.Classes.
 
   Module Import RewriteRules.
@@ -23,8 +23,8 @@ Module Compilers.
               (Hlow : forall s v v', invert_low s v = Some v' -> v = Z.land v' (2^(s/2)-1))
               (Hhigh : forall s v v', invert_high s v = Some v' -> v = Z.shiftr v' (s/2)).
 
-      Definition VerifiedRewriterToFancyWithCasts : VerifiedRewriter.
-      Proof using All. make_rewriter false (@fancy_with_casts_rewrite_rules_proofs invert_low invert_high value_range flag_range Hlow Hhigh). Defined.
+      Definition VerifiedRewriterToFancyWithCasts : VerifiedRewriter_with_args false (@fancy_with_casts_rewrite_rules_proofs invert_low invert_high value_range flag_range Hlow Hhigh).
+      Proof using All. make_rewriter. Defined.
 
       Definition RewriteToFancyWithCasts {t} : API.Expr t -> API.Expr t.
       Proof using invert_low invert_high value_range flag_range.
